remove the well-formedness requirement on tags

theories/stacked_borrows/defs.v
@@ -36,7 +36,7 @@ Definition wf_scalar t sc := ∀ t' l, sc = ScPtr l t' → t' <t t.
 
 Record state_wf (s: state) := {
   state_wf_dom : dom (gset loc) s.(shp) ≡ dom (gset loc) s.(sst);
-  state_wf_mem_tag : wf_mem_tag s.(shp) s.(snp);
+  (*state_wf_mem_tag : wf_mem_tag s.(shp) s.(snp);*)
   state_wf_stack_item : wf_stacks s.(sst) s.(snp) s.(snc);
   state_wf_non_empty : wf_non_empty s.(sst);
   (*state_wf_cid_no_dup : NoDup s.(scs) ;*)
